doc/tutorial/code/exercises/Ex12d.Pad.fst
@@ -25,32 +25,34 @@ type uint8 = FStar.UInt8.t
 assume val n2b: n:nat {( n < 256 )} -> Tot uint8
 assume val b2n: b:uint8 -> Tot (n:nat { (n < 256) /\ n2b n = b })
 
-type bytes = seq byte (* concrete byte arrays *) 
+type bytes = seq byte (* concrete byte arrays *)
 type nbytes (n:nat) = b:bytes{length b == n} (* fixed-length bytes *)
 
-let blocksize = 32 
+let blocksize = 32
 type block = nbytes blocksize
 type text = b:bytes {(length b < blocksize)}
 
 // BEGIN: PadEx
 (* fill in type here and remove the assumption*)
-let pad (n:int) =
-  assume (1 <= n /\ n < 256);
-  Seq.create n (n2b (n-1))  
+val pad: n:int{n > 0 /\ n < 256} -> bytes
+let pad n =
+  Seq.create n (n2b (n-1))
 
 (* pad 1 = [| 0 |]; pad 2 = [| 1; 1 |]; ... *)
 
 (* fill in type here *)
+val encode: a:bytes{length a > 0 /\ length a < blocksize} -> bytes
 let encode a = append a (pad (blocksize - length a))
 
 
 (* fill in type here *)
-let decode (b:block) = 
+val decode: block -> b:option bytes{b2t(Some? b) ==> b2t(let Some b' = b in length b' > 0 && length b' < blocksize)}
+let decode b =
   let padsize = b2n(index b (blocksize - 1)) + 1 in
-  if op_LessThan padsize blocksize then 
+  if op_LessThan padsize blocksize then
     let (plain,padding) = split b (blocksize - padsize) in
     if  Seq.eq padding (pad padsize)
     then Some plain
-    else None   
+    else None
   else None
 // END: PadEx
